{
 "cells": [
  {
   "cell_type": "code",
   "execution_count": 2,
   "id": "21b37b0b-193a-4fbd-9f3a-e88ae94edbbe",
   "metadata": {
    "scrolled": true,
    "tags": []
   },
   "outputs": [],
   "source": [
    "# Find the value of T(2) for the recurrence relation T(n) = 3T(n-1) + 12n, given that T(0) = 5.\n",
    "\n",
    "# Recurrence Relation:\n",
    "# T(n) = 3T(n-1) + 12n\n",
    "\n",
    "# Initial Condition:\n",
    "# T(0) = 5\n",
    "\n",
    "# Calculate T(1):\n",
    "#T(1) = 3 * T(0) + 12 * 1\n",
    "     # = 3 * 5 + 12\n",
    "    #  = 27\n",
    "\n",
    "# Calculate T(2):\n",
    "#T(2) = 3 * T(1) + 12 * 2\n",
    "    #  = 3 * 27 + 24\n",
    "      #= 105\n",
    "\n",
    "# Therefore, the value of T(2) for the given recurrence relation is 105.\n",
    "\n",
    "\n",
    "#2 Given a recurrence relation, solve it using the substitution method:\n",
    "\n",
    "# a. T(n) = T(n-1) + c\n",
    "\n",
    "# Substitution method\n",
    "# T(n) = T(n-1) + c\n",
    "\n",
    "# Assumption: T(k) = T(k-1) + c\n",
    "# Substitute: T(n) = T(n-2) + 2c\n",
    "# Repeat until base case (assume base case is T(0))\n",
    "\n",
    "# T(n) = T(0) + nc\n",
    "\n",
    "# b. T(n) = 2T(n/2) + n\n",
    "\n",
    "# Substitution method\n",
    "# T(n) = 2T(n/2) + n\n",
    "\n",
    "# Assumption: T(k) = 2T(k/2) + k\n",
    "# Substitute: T(n) = 2^2 T(n/2^2) + n + n\n",
    "# Repeat until base case (assume base case is T(1))\n",
    "\n",
    "#T(n) = 2^(log2(n)) T(1) + n log2(n)\n",
    "\n",
    "\n",
    "# c. T(n) = 2T(n/2) + c\n",
    "\n",
    "# Substitution method\n",
    "# T(n) = 2T(n/2) + c\n",
    "\n",
    "# Assumption: T(k) = 2T(k/2) + c\n",
    "# Substitute: T(n) = 2^2 T(n/2^2) + 2c\n",
    "# Repeat until base case (assume base case is T(1))\n",
    "\n",
    "#T(n) = 2^(log2(n)) T(1) + c (log2(n) - 1)\n",
    "\n",
    "\n",
    "# d. T(n) = T(n/2) + c\n",
    "\n",
    "# Substitution method\n",
    "# T(n) = T(n/2) + c\n",
    "\n",
    "# Assumption: T(k) = T(k/2) + c\n",
    "# Substitute: T(n) = T(n/2^2) + 2c\n",
    "# Repeat until base case (assume base case is T(1))\n",
    "\n",
    "#T(n) = T(1) + c log2(n)\n",
    "\n",
    "# 3. Given a recurrence relation, solve it using the recursive tree approach:\n",
    "\n",
    "# a. T(n) = 2T(n-1) + 1\n",
    "\n",
    "# Recursive Tree Approach:\n",
    "# Start with T(n).\n",
    "# At each level, multiply by the coefficient of the recurrence term (2) and add the constant term (1).\n",
    "# Continue this process until reaching the base case.\n",
    "\n",
    "# Step 1:\n",
    "# T(n) = 2T(n-1) + 1\n",
    "\n",
    "# Step 2:\n",
    "# T(n) = 2[2T(n-2) + 1] + 1\n",
    "\n",
    "# In general:\n",
    "# T(n) = 2^(n-1) T(1) + (n-1)\n",
    "\n",
    "# b. T(n) = 2T(n/2) + n\n",
    "\n",
    "# Recursive Tree Approach:\n",
    "# Start with T(n).\n",
    "# At each level, multiply by the coefficient of the recurrence term (2) and add the constant term (n).\n",
    "# Continue this process until reaching the base case.\n",
    "\n",
    "# Step 1:\n",
    "# T(n) = 2T(n/2) + n\n",
    "\n",
    "# Step 2:\n",
    "# T(n) = 2[2T(n/4) + n/2] + n\n",
    "\n",
    "# In general:\n",
    "# T(n) = n log2(n) + n"
   ]
  },
  {
   "cell_type": "code",
   "execution_count": null,
   "id": "3a4dd572-97f7-4012-ab9b-f17ca1df6510",
   "metadata": {},
   "outputs": [],
   "source": []
  },
  {
   "cell_type": "code",
   "execution_count": null,
   "id": "005a03ea-d081-4618-847c-3e3cb966c909",
   "metadata": {},
   "outputs": [],
   "source": []
  }
 ],
 "metadata": {
  "kernelspec": {
   "display_name": "Python 3 (ipykernel)",
   "language": "python",
   "name": "python3"
  },
  "language_info": {
   "codemirror_mode": {
    "name": "ipython",
    "version": 3
   },
   "file_extension": ".py",
   "mimetype": "text/x-python",
   "name": "python",
   "nbconvert_exporter": "python",
   "pygments_lexer": "ipython3",
   "version": "3.10.8"
  }
 },
 "nbformat": 4,
 "nbformat_minor": 5
}
